cleanup

Map.lean
@@ -1,13 +1,13 @@
 import Init.Data.Int.Basic
 
-inductive Map (α β : Type) [Ord α] [Hashable α] where
+inductive Map (α β : Type) [Hashable α] where
   | empty : Map α β
   | node : Map α β → (UInt64 × β) → Map α β → Map α β
   deriving Repr
 
 namespace Map
 
-def getOption {α β : Type} [Ord α] [Hashable α] : α → Map α β → Option β
+def getOption {α β : Type} [Hashable α] : α → Map α β → Option β
 | _, empty => Option.none
 | x, node left (y, value) right =>
   match Ord.compare (Hashable.hash x) y with
@@ -15,24 +15,24 @@ def getOption {α β : Type} [Ord α] [Hashable α] : α → Map α β → Optio
   | Ordering.lt => getOption x left
   | Ordering.gt => getOption x right
 
-def insert {α β : Type} [Ord α] [Hashable α] : α → β → Map α β → Map α β
-| x, y, empty => node empty (Hashable.hash x, y) empty
-| x, y, node left (key, value) right =>
+def insert {α β : Type} [Hashable α] : Map α β → α → β → Map α β
+| empty, x, y => node empty (Hashable.hash x, y) empty
+| node left (key, value) right, x, y =>
   let
     hashed := Hashable.hash x
   match Ord.compare hashed key with
   | Ordering.eq => node left (hashed, y) right
-  | Ordering.lt => node (insert x y left) (key, value) right
-  | Ordering.gt => node left (key, value) (insert x y right)
+  | Ordering.lt => node (left.insert x y) (key, value) right
+  | Ordering.gt => node left (key, value) (right.insert x y)
 
-def Mem [Ord α] [Hashable α] (x : α) : Map α β → Prop
+def Mem [Hashable α] (x : α) : Map α β → Prop
   | .empty => False
   | .node left (y, _) right => (Hashable.hash x = y) ∨ (Mem x left) ∨ (Mem x right)
 
-instance [Ord α] [Hashable α] : Membership α (Map α β) where
+instance [Hashable α] : Membership α (Map α β) where
   mem := Mem
 
-instance Mem.decidableMap [DecidableEq α] [Ord α] [Hashable α] (x : α) : ∀ xs : Map α β, Decidable (x ∈ xs)
+instance Mem.decidableMap [DecidableEq α] [Hashable α] (x : α) : ∀ xs : Map α β, Decidable (x ∈ xs)
   | empty => by
     apply Decidable.isFalse
     simp [Membership.mem, Mem]
@@ -54,7 +54,7 @@ theorem Or.elimLeft (xs : α ∨ β) (x: ¬α) : β :=
   | Or.inl y => absurd y x
   | Or.inr b => b
 
-def get {α β : Type} [DecidableEq α] [Ord α] [Hashable α] : (x : α) → { xs : Map α β // x ∈ xs } → β
+def get {α β : Type} [DecidableEq α] [Hashable α] : (x : α) → { xs : Map α β // x ∈ xs } → β
   | x, ⟨node left (y, v) right, ok⟩ =>
     let hashed := Hashable.hash x
     if here : hashed = y then
@@ -65,32 +65,32 @@ def get {α β : Type} [DecidableEq α] [Ord α] [Hashable α] : (x : α) → { 
       else
         get x ⟨ right, Map.Or.elimLeft (Map.Or.elimLeft ok here) l ⟩
 
-def ofList [Hashable α] [Ord α] : List (α × β) → Map α β
+def ofList [Hashable α] : List (α × β) → Map α β
 | [] => empty
 | (x, y) :: rest =>
-  insert x y (ofList rest)
+  (ofList rest).insert x y
 
-instance [Hashable α] [Ord α] : Coe (List (α × β)) (Map α β) where
+instance [Hashable α] : Coe (List (α × β)) (Map α β) where
   coe := ofList
 
-theorem belongIff [Ord α] [Hashable α] {x : α} {xs : Map α β} : x ∈ xs ↔ Mem x xs := by
+theorem belongIff [Hashable α] {x : α} {xs : Map α β} : x ∈ xs ↔ Mem x xs := by
   simp [(·∈·)];
 
-theorem belongs {α β : Type} [Ord α] [Hashable α] {y : β} {left right : Map α β} : ∀ {x : α}, x ∈ node left (hash x, y) right := by
+theorem belongs {α β : Type} [Hashable α] {y : β} {left right : Map α β} : ∀ {x : α}, x ∈ node left (hash x, y) right := by
   intro x;
   simp [(·∈·), Mem];
 
-theorem belongsL {α β : Type} [Ord α] [Hashable α] { n : UInt64 × β } {left right : Map α β} : ∀ {x : α}, x ∈ left → x ∈ node left n right := by
+theorem belongsL {α β : Type} [Hashable α] { n : UInt64 × β } {left right : Map α β} : ∀ {x : α}, x ∈ left → x ∈ node left n right := by
   intro x
   intro belong
   simp [(·∈·), Mem, Iff.mp belongIff belong]
 
-theorem belongsR {α β : Type} [Ord α] [Hashable α] { n : UInt64 × β } {left right : Map α β} : ∀ {x : α}, x ∈ right → x ∈ node left n right := by
+theorem belongsR {α β : Type} [Hashable α] { n : UInt64 × β } {left right : Map α β} : ∀ {x : α}, x ∈ right → x ∈ node left n right := by
   intro x
   intro belong
   simp [(·∈·), Mem, Iff.mp belongIff belong]
 
-def insertP {α β : Type} [Ord α] [Hashable α] : (x : α) → β → Map α β → { xs : Map α β // x ∈ xs }
+def insertP {α β : Type} [Hashable α] : (x : α) → β → Map α β → { xs : Map α β // x ∈ xs }
 | x, y, empty => ⟨ node empty (Hashable.hash x, y) empty, belongs ⟩
 | x, y, node left (key, value) right =>
   let
@@ -109,7 +109,7 @@ def insertP {α β : Type} [Ord α] [Hashable α] : (x : α) → β → Map α �
     | ⟨ r, p ⟩ =>
       ⟨ node left (key, value) r, belongsR p ⟩
 
-instance [Ord α] [Hashable α] [DecidableEq α] : GetElem (Map α β) α β (λ map elem => elem ∈ map) where
+instance [Hashable α] [DecidableEq α] : GetElem (Map α β) α β (λ map elem => elem ∈ map) where
   getElem map elem proof := get elem ⟨ map, proof ⟩
 
 end Map
