Rinha.lean
@@ -1,2 +1,1 @@
-import Rinha.Environment
 import Rinha.Term
